src/Layer1/HoareLogic.v
@@ -1,190 +1,18 @@
 Require Import Primitives Simulation Layer1.Definitions ProgAuto.
 
-Set Implicit Arguments.
+Module Layer1 <: Layer.
+  Definition oracle := oracle.
+  Definition data := set value.
+  Definition prog := prog.
+  Definition exec := exec.
+  Definition oracle_ok := (fun T => @oracle_ok T).
+End Layer1.
 
+Module Layer1HL := HoareLogic Layer1.
+Export Layer1.
+Export Layer1HL.
 
-(** ** Hoare logic *)
-Definition precond := oracle -> @pred addr addr_dec (set value).
-Definition postcond {T: Type} := T -> @pred addr addr_dec (set value).
-Definition crashcond := @pred addr addr_dec (set value).
-Definition augpostcond {T: Type} := oracle -> disk (set value) -> T -> @pred addr addr_dec (set value).
-Definition augcrashcond := oracle -> disk (set value) -> @pred addr addr_dec (set value).
-
-Definition hoare_triple {T: Type} (pre: precond) (p: prog T) (post: @postcond T) (crash: crashcond) (augpost: augpostcond) (augcrash: augcrashcond):=
-  fun o d =>
-    pre o d ->
-    (exists ret,
-        exec o d p ret /\
-        ((exists d' r,
-             ret = Finished d' r
-             /\ post r d' /\ augpost o d r d') \/
-         (exists d',
-             ret = Crashed d' /\ crash d' /\ augcrash o d d')))%type.
-
-
-  
-Notation
-  "<< o , d >> pre p << r >> post crash" :=
-  (forall F, hoare_triple
-          (fun o d => (F * pre * [[ oracle_ok p o d ]]) d)%pred
-          p%pred
-          (fun r => F * post)%pred
-          (F * crash)%pred
-          (fun _ _ _ => any)
-          (fun _ _ => any)
-          o d)      
-    (at level 10, o at next level, d at next level, pre at next level, p at next level, r at next level, post at next level, crash at next level,
-     format "'[v' '[  ' '<<' o ','  d '>>' '//' '[' pre ']' '//' '[' p ']' ']' '//' '[  ' '<<' r '>>' '//' '[' post ']' '//' '[' crash ']' ']' ']'").
-
-Notation
-  "<< o , d >> pre p << r >> post crash augpost augcrash" :=
-  (forall F, hoare_triple
-          (fun o d => (F * pre * [[ oracle_ok p o d ]]) d)%pred
-          p%pred
-          (fun r => F * post)%pred
-          (F * crash)%pred
-          (fun o d r => F * augpost)%pred
-          (fun o d => F * augcrash)%pred
-          o d)      
-    (at level 10, o at next level, d at next level, pre at next level, p at next level, r at next level, post at next level, crash at next level, augpost at next level, augcrash at next level,
-     format "'[v' '[  ' '<<' o ','  d '>>' '//' '[' pre ']' '//' '[' p ']' ']' '//' '[  ' '<<' r '>>' '//' '[' post ']' '//' '[' crash ']' '//' '[' augpost ']' '//' '[' augcrash ']' ']' ']'").
-
-(*
-Notation
-  "{{ e1 }} << o >> pre p << r >> post crash" :=
-   (exists e1, (forall F, hoare_triple
-          (fun o => F * pre)%pred
-          p
-          (fun r => F * post)%pred
-          (F * crash)%pred))
-    (at level 10, o at next level, pre at next level, p at next level, r at next level, post at next level, crash at next level,
-     format "'[v' '{{' e1 '}}' '//' '[  ' '<<' o '>>' '//' pre '//' p ']' '//' '[  ' '<<' r '>>' '//' post '//' crash ']' ']'").
-*)
-
-(*
-Theorem hoare_triple_strengthen_pre:
-  forall T (p: prog T) (pre pre': precond) post crash,
-  hoare_triple pre p post crash ->
-  (forall o, pre' o =p=>  pre o) ->
-  hoare_triple pre' p post crash.
-Proof.
-  unfold hoare_triple; intros;
-    edestruct H; intros; eauto.
-  eapply H0; eauto.
-Qed.
-
-Theorem hoare_triple_weaken_post_weak:
-  forall T (p: prog T) pre (post post': postcond) crash,
-  hoare_triple pre p post crash ->
-  (forall  o d r,
-      pre o d ->
-      post r =p=>
-      post' r) ->
-  hoare_triple pre p post' crash.
-Proof.
-  unfold hoare_triple; intros;
-    edestruct H; intros; eauto.
-  cleanup; split_ors; cleanup.
-  eexists; split; eauto.  
-  left; repeat eexists; eauto.
-  eapply H0; eauto.
-  eexists; split; eauto.
-Qed.
-
-
-Theorem hoare_triple_weaken_post_strong:
-  forall T (p: prog T) pre (post post': postcond) crash,
-  hoare_triple pre p post crash ->
-  (forall o d (r: T),
-      post o d r =p=>
-      post' o d r) ->
-  hoare_triple pre p post' crash.
-Proof.
-  intros; eapply hoare_triple_weaken_post_weak; eauto.
-Qed.
-
-Theorem hoare_triple_weaken_crash_weak:
-  forall T (p: prog T) pre post (crash crash': crashcond),
-  hoare_triple pre p post crash ->
-  (forall o d,
-      pre o d ->
-      crash o d =p=>
-      crash' o d) ->
-  hoare_triple pre p post crash'.
-Proof.
-  unfold  hoare_triple; intros;
-    edestruct H; intros; eauto.
-  cleanup; split_ors; cleanup.
-  eexists; split; eauto.
-  eexists; split; eauto.  
-  right; repeat eexists; eauto.
-  eapply H0; eauto. 
-Qed.
-
-
-Theorem hoare_triple_weaken_crash_strong:
-  forall T (p: prog T) pre post (crash crash': crashcond),
-  hoare_triple pre p post crash ->
-  (forall o d, crash o d =p=> crash' o d) ->
-  hoare_triple pre p post crash'.
-Proof.
-  intros; eapply hoare_triple_weaken_crash_weak; eauto.
-Qed.
-
-
-Theorem hoare_triple_pimpl :
-    forall T1 T2 (p1: prog T1) (p2: T1 -> prog T2) (pre: precond) pre1 post1 pre2 post2 crash1 crash2,
-      hoare_triple pre1 p1 post1 crash1 ->
-      (forall o d,
-          pre o d ->
-          exists o1 o2,
-            o = o1++o2 /\
-            (o2 = [] \/ ~In Crash o1) /\
-            pre1 o1 d) ->
-      (forall o1 d,
-         pre1 o1 d ->
-         (forall o2 r, post1 r =p=> pre2 o2)) ->
-      (forall o1 d r,
-         pre1 o1 d ->
-         (forall o2, post1 r =p=> pre2 o2) ->
-          hoare_triple pre2 (p2 r) post2 crash2) ->
-    (forall o d,
-      pre1 o d ->
-      crash1 =p=> crash2) ->
-    hoare_triple pre (Bind p1 p2) post2 crash2.
-Proof.
-  unfold hoare_triple; intros.
-  edestruct H0; eauto; cleanup.
-  edestruct H; eauto; cleanup.
-  specialize H1 with (1:=H7).
-  specialize H3 with (1:=H7).
-  split_ors.
-  - (* p1 Finished *)    
-    edestruct H2; eauto.
-    eapply H1; eauto.
-    cleanup.
-    split_ors; cleanup.
-    + (* p2 Finished *)
-      clear H8.
-      eexists; split; eauto.
-      left; do 2 eexists; intuition eauto.
-      eapply H4; eauto.
-      eapply H1; eauto.
-    + (* p2 Crashed *)
-      clear H8.
-      eexists. intuition eauto.
-      right; eexists; intuition eauto.
-      eapply H5; eauto.
-      eapply H1; eauto.
-  - (* p1 Crashed *)
-    split_ors; cleanup.
-    eexists. intuition eauto.
-    cleanup; rewrite app_nil_r;
-      econstructor; eauto.
-    cleanup; rewrite app_nil_r; eauto.
-    apply exec_crash_in in H7; intuition.   
-Qed.
-*)
+Arguments exec {T}.
 
 Theorem hoare_triple_equivalence :
   forall T (p p': prog T) o d pre post crash ap ac,
@@ -198,31 +26,8 @@ Proof.
   | [ H: _ ~= _ |- _ ] =>
     edestruct H; eauto
   end.
-Qed.
-
-Theorem remember_oracle_ok :
-  forall T (p: prog T) o d pre post crash ap ac,
-    (oracle_ok p o d ->
-  << o, d >>
-   pre
-   p
-  << r >>
-   (post r)
-   crash
-   (ap o d r)
-   (ac o d)) ->
-  << o, d >>
-   pre
-   p
-  << r >>
-   (post r)
-   crash
-   (ap o d r)
-   (ac o d).
-Proof.
-  unfold hoare_triple; intros.
-  eapply H; eauto.
-  destruct_lift  H0; eauto.
+  unfold exec in *.
+  eauto.
 Qed.
 
 Ltac monad_simpl_one :=
@@ -233,6 +38,7 @@ Ltac monad_simpl_one :=
   end.
 
 Ltac monad_simpl := repeat monad_simpl_one.
+
 
 Theorem bind_ok:
   forall T T' (p1: prog T) (p2: T -> prog T') pre1 post1 crash1 pre2 post2 crash2 pre3 post3 crash3 o d,
@@ -278,7 +84,7 @@ Theorem bind_ok:
      (post3 r)
      crash3.
 Proof.
-  unfold hoare_triple; intros.
+  unfold hoare_triple, exec; intros.
   simpl in *; destruct_lifts; cleanup.
   rewrite H0 in H6.
   edestruct H; eauto.
@@ -313,224 +119,6 @@ Proof.
     pred_apply' H12; cancel.
     eauto.
 Qed.
-
-
-Theorem crash_weaken:
-  forall T (p: prog T) pre post crash1 crash2 o d,
-  << o, d >>
-   pre
-   p
-  << r >>
-   (post r)
-   crash1 ->
-  (crash1 =p=> crash2) ->
-  << o, d >>
-     pre
-     p
-  << r >>
-     (post r)
-     crash2.
-Proof.
-  unfold hoare_triple; intros.
-  edestruct H; eauto.
-  cleanup.
-  split_ors; cleanup;
-    eexists; intuition eauto.
-  right; eexists; intuition eauto.
-  clear H5; pred_apply; cancel; eauto.
-Qed.
-
-
-Theorem post_weaken:
-  forall T (p: prog T) pre post1 post2 crash o d,
-  << o, d >>
-   pre
-   p
-  << r >>
-   (post1 r)
-   crash  ->
-  (forall r, post1 r =p=> post2 r) ->
-  << o, d >>
-     pre
-     p
-  << r >>
-     (post2 r)
-     crash.
-Proof.
-  unfold hoare_triple; intros.
-  edestruct H; eauto.
-  cleanup.
-  split_ors; cleanup;
-    eexists; intuition eauto.
-  left; do 2 eexists; intuition eauto.
-  clear H5; pred_apply; cancel; eauto.
-Qed.
-
-Theorem pre_strengthen:
-  forall T (p: prog T) pre1 pre2 post crash o d,
-  << o, d >>
-   pre1
-   p
-  << r >>
-   (post r)
-   crash ->
-  (pre2 =p=> pre1) ->
-  << o, d >>
-     pre2
-     p
-  << r >>
-     (post r)
-     crash.
-Proof.
-  unfold hoare_triple; intros.
-  edestruct H; eauto.
-  pred_apply; cancel; eauto.
-Qed.
-
-Theorem pre_strengthen_aug:
-  forall T (p: prog T) pre1 pre2 post crash ap ac o d,
-  << o, d >>
-   pre1
-   p
-  << r >>
-   (post r)
-   crash
-   (ap o d r)
-   (ac o d) ->
-  (pre2 =p=> pre1) ->
-  << o, d >>
-     pre2
-     p
-  << r >>
-     (post r)
-     crash
-     (ap o d r)
-     (ac o d).
-Proof.
-  unfold hoare_triple; intros.
-  edestruct H; eauto.
-  pred_apply; cancel; eauto.
-Qed.
-
-
-Theorem add_frame:
-  forall T (p: prog T) pre post crash F o d,
-  << o, d >>
-   pre
-   p
-  << r >>
-   (post r)
-   crash  ->
-  << o, d >>
-     (F * pre)
-     p
-  << r >>
-     (F * post r)
-     (F * crash).
-Proof.
-  unfold hoare_triple; intros.
-  edestruct H; eauto.
-  pred_apply' H0; cancel; eauto.
-  cleanup; split_ors; cleanup;
-    eexists; intuition eauto.
-  left; do 2 eexists; intuition eauto.
-  clear H4; pred_apply; cancel; eauto.
-  right; eexists; intuition eauto.
-  clear H4; pred_apply; cancel; eauto.
-Qed.
-
-Theorem extract_exists:
-  forall T V (p: prog T) pre post crash o d,
-    (forall (v:V),
-  << o, d >>
-   (pre v)
-   p
-  << r >>
-   (post r)
-   crash) ->
-  << o, d >>
-     (exists v, pre v)
-     p
-  << r >>
-     (post r)
-     crash.
-Proof.
-  unfold hoare_triple; intros.
-  destruct_lifts.
-  eapply H; eauto.
-  pred_apply' H0; cancel; eauto.
-Qed.
-
-Theorem extract_exists_aug:
-  forall T V (p: prog T) pre post crash ap ac o d,
-    (forall (v:V),
-  << o, d >>
-   (pre v)
-   p
-  << r >>
-   (post r)
-   crash
-   (ap o d r)
-   (ac o d)) ->
-  << o, d >>
-     (exists v, pre v)
-     p
-  << r >>
-     (post r)
-     crash
-     (ap o d r)
-     (ac o d).
-Proof.
-  unfold hoare_triple; intros.
-  destruct_lifts.
-  eapply H; eauto.
-  pred_apply' H0; cancel; eauto.
-Qed.
-
-Theorem remove_augcons:
-  forall T (p: prog T) pre post crash (augpost: augpostcond) (augcrash: augcrashcond) o d,
-  << o, d >>
-   pre
-   p
-  << r >>
-   (post r)
-   crash ->
-  (forall F d' r,
-      (F * pre)%pred d ->
-      exec o d p (Finished d' r) ->
-      (F * post r)%pred d' ->
-      (F * augpost o d r)%pred d') ->
-  (forall F d',
-      (F * pre)%pred d ->
-      exec o d p (Crashed d') ->
-      (F * crash)%pred d' ->
-      (F * augcrash o d)%pred d') ->
-  << o, d >>
-     pre
-     p
-  << r >>
-     (post r)
-     crash
-     (augpost o d r)
-     (augcrash o d).
-Proof.
-  unfold hoare_triple; intros.
-  edestruct H; eauto; cleanup.
-  
-  split_ors; cleanup.
-  - 
-    eexists; split; intuition eauto.
-    left; do 2 eexists; intuition eauto.
-    eapply H0; eauto.
-    pred_apply; cancel.
-    
-  - 
-    eexists; split; intuition eauto.
-    right; eexists; intuition eauto.
-    eapply H1; eauto.
-    pred_apply; cancel.
-Qed.
-
 
 Theorem bind_ok_aug:
   forall T T' (p1: prog T) (p2: T -> prog T') pre1 post1 crash1 pre2 post2 crash2 pre3 post3 crash3 augpost augcrash o d,
@@ -589,7 +177,7 @@ Theorem bind_ok_aug:
      (augcrash o d)
      .
 Proof.
-  unfold hoare_triple; intros.
+  unfold hoare_triple, exec; intros.
   simpl in *; destruct_lifts; cleanup.
   rewrite H0 in H7.
   edestruct H; eauto.
