src/Common/HoareLogic.v
@@ -1,0 +1,315 @@
+Require Import BaseTypes Mem Pred Disk CommonAutomation SepAuto.
+
+Set Implicit Arguments.
+
+Module Type Layer.
+  Parameter oracle : Type.
+  Parameter data : Type.
+  Parameter prog : Type -> Type.
+  Parameter exec: forall T, oracle -> disk data -> prog T -> @Result (disk data) T -> Prop.
+  Parameter oracle_ok : forall T, prog T -> oracle -> disk data -> Prop.
+End Layer.
+
+Module HoareLogic (l: Layer).
+  Import l.
+(** ** Hoare logic *)
+Definition precond := oracle -> @pred addr addr_dec data.
+Definition postcond {T: Type} := T -> @pred addr addr_dec data.
+Definition crashcond := @pred addr addr_dec data.
+Definition augpostcond {T: Type} := oracle -> disk data -> T -> @pred addr addr_dec data.
+Definition augcrashcond := oracle -> disk data -> @pred addr addr_dec data.
+
+Definition hoare_triple {T: Type} (pre: precond) (p: prog T) (post: @postcond T) (crash: crashcond) (augpost: augpostcond) (augcrash: augcrashcond):=
+  fun o d =>
+    pre o d ->
+    (exists ret,
+        exec o d p ret /\
+        ((exists d' r,
+             ret = Finished d' r
+             /\ post r d' /\ augpost o d r d') \/
+         (exists d',
+             ret = Crashed d' /\ crash d' /\ augcrash o d d')))%type.
+
+
+  
+Notation
+  "<< o , d >> pre p << r >> post crash" :=
+  (forall F, hoare_triple
+          (fun o d => (F * pre * [[ oracle_ok p o d ]]) d)%pred
+          p%pred
+          (fun r => F * post)%pred
+          (F * crash)%pred
+          (fun _ _ _ => any)
+          (fun _ _ => any)
+          o d)      
+    (at level 10, o at next level, d at next level, pre at next level, p at next level, r at next level, post at next level, crash at next level,
+     format "'[v' '[  ' '<<' o ','  d '>>' '//' '[' pre ']' '//' '[' p ']' ']' '//' '[  ' '<<' r '>>' '//' '[' post ']' '//' '[' crash ']' ']' ']'").
+
+Notation
+  "<< o , d >> pre p << r >> post crash augpost augcrash" :=
+  (forall F, hoare_triple
+          (fun o d => (F * pre * [[ oracle_ok p o d ]]) d)%pred
+          p%pred
+          (fun r => F * post)%pred
+          (F * crash)%pred
+          (fun o d r => F * augpost)%pred
+          (fun o d => F * augcrash)%pred
+          o d)      
+    (at level 10, o at next level, d at next level, pre at next level, p at next level, r at next level, post at next level, crash at next level, augpost at next level, augcrash at next level,
+     format "'[v' '[  ' '<<' o ','  d '>>' '//' '[' pre ']' '//' '[' p ']' ']' '//' '[  ' '<<' r '>>' '//' '[' post ']' '//' '[' crash ']' '//' '[' augpost ']' '//' '[' augcrash ']' ']' ']'").
+
+(*
+Notation
+  "{{ e1 }} << o >> pre p << r >> post crash" :=
+   (exists e1, (forall F, hoare_triple
+          (fun o => F * pre)%pred
+          p
+          (fun r => F * post)%pred
+          (F * crash)%pred))
+    (at level 10, o at next level, pre at next level, p at next level, r at next level, post at next level, crash at next level,
+     format "'[v' '{{' e1 '}}' '//' '[  ' '<<' o '>>' '//' pre '//' p ']' '//' '[  ' '<<' r '>>' '//' post '//' crash ']' ']'").
+*)
+
+Theorem remember_oracle_ok :
+  forall T (p: prog T) o d pre post crash ap ac,
+    (oracle_ok p o d ->
+  << o, d >>
+   pre
+   p
+  << r >>
+   (post r)
+   crash
+   (ap o d r)
+   (ac o d)) ->
+  << o, d >>
+   pre
+   p
+  << r >>
+   (post r)
+   crash
+   (ap o d r)
+   (ac o d).
+Proof.
+  unfold hoare_triple; intros.
+  eapply H; eauto.
+  destruct_lift  H0; eauto.
+Qed.
+
+
+Theorem crash_weaken:
+  forall T (p: prog T) pre post crash1 crash2 o d,
+  << o, d >>
+   pre
+   p
+  << r >>
+   (post r)
+   crash1 ->
+  (crash1 =p=> crash2) ->
+  << o, d >>
+     pre
+     p
+  << r >>
+     (post r)
+     crash2.
+Proof.
+  unfold hoare_triple; intros.
+  edestruct H; eauto.
+  cleanup.
+  split_ors; cleanup;
+    eexists; intuition eauto.
+  right; eexists; intuition eauto.
+  clear H5; pred_apply; cancel; eauto.
+Qed.
+
+
+Theorem post_weaken:
+  forall T (p: prog T) pre post1 post2 crash o d,
+  << o, d >>
+   pre
+   p
+  << r >>
+   (post1 r)
+   crash  ->
+  (forall r, post1 r =p=> post2 r) ->
+  << o, d >>
+     pre
+     p
+  << r >>
+     (post2 r)
+     crash.
+Proof.
+  unfold hoare_triple; intros.
+  edestruct H; eauto.
+  cleanup.
+  split_ors; cleanup;
+    eexists; intuition eauto.
+  left; do 2 eexists; intuition eauto.
+  clear H5; pred_apply; cancel; eauto.
+Qed.
+
+Theorem pre_strengthen:
+  forall T (p: prog T) pre1 pre2 post crash o d,
+  << o, d >>
+   pre1
+   p
+  << r >>
+   (post r)
+   crash ->
+  (pre2 =p=> pre1) ->
+  << o, d >>
+     pre2
+     p
+  << r >>
+     (post r)
+     crash.
+Proof.
+  unfold hoare_triple; intros.
+  edestruct H; eauto.
+  pred_apply; cancel; eauto.
+Qed.
+
+Theorem pre_strengthen_aug:
+  forall T (p: prog T) pre1 pre2 post crash ap ac o d,
+  << o, d >>
+   pre1
+   p
+  << r >>
+   (post r)
+   crash
+   (ap o d r)
+   (ac o d) ->
+  (pre2 =p=> pre1) ->
+  << o, d >>
+     pre2
+     p
+  << r >>
+     (post r)
+     crash
+     (ap o d r)
+     (ac o d).
+Proof.
+  unfold hoare_triple; intros.
+  edestruct H; eauto.
+  pred_apply; cancel; eauto.
+Qed.
+
+
+Theorem add_frame:
+  forall T (p: prog T) pre post crash F o d,
+  << o, d >>
+   pre
+   p
+  << r >>
+   (post r)
+   crash  ->
+  << o, d >>
+     (F * pre)
+     p
+  << r >>
+     (F * post r)
+     (F * crash).
+Proof.
+  unfold hoare_triple; intros.
+  edestruct H; eauto.
+  pred_apply' H0; cancel; eauto.
+  cleanup; split_ors; cleanup;
+    eexists; intuition eauto.
+  left; do 2 eexists; intuition eauto.
+  clear H4; pred_apply; cancel; eauto.
+  right; eexists; intuition eauto.
+  clear H4; pred_apply; cancel; eauto.
+Qed.
+
+Theorem extract_exists:
+  forall T V (p: prog T) pre post crash o d,
+    (forall (v:V),
+  << o, d >>
+   (pre v)
+   p
+  << r >>
+   (post r)
+   crash) ->
+  << o, d >>
+     (exists v, pre v)
+     p
+  << r >>
+     (post r)
+     crash.
+Proof.
+  unfold hoare_triple; intros.
+  destruct_lifts.
+  eapply H; eauto.
+  pred_apply' H0; cancel; eauto.
+Qed.
+
+Theorem extract_exists_aug:
+  forall T V (p: prog T) pre post crash ap ac o d,
+    (forall (v:V),
+  << o, d >>
+   (pre v)
+   p
+  << r >>
+   (post r)
+   crash
+   (ap o d r)
+   (ac o d)) ->
+  << o, d >>
+     (exists v, pre v)
+     p
+  << r >>
+     (post r)
+     crash
+     (ap o d r)
+     (ac o d).
+Proof.
+  unfold hoare_triple; intros.
+  destruct_lifts.
+  eapply H; eauto.
+  pred_apply' H0; cancel; eauto.
+Qed.
+
+Theorem remove_augcons:
+  forall T (p: prog T) pre post crash (augpost: augpostcond) (augcrash: augcrashcond) o d,
+  << o, d >>
+   pre
+   p
+  << r >>
+   (post r)
+   crash ->
+  (forall F d' r,
+      (F * pre)%pred d ->
+      exec o d p (Finished d' r) ->
+      (F * post r)%pred d' ->
+      (F * augpost o d r)%pred d') ->
+  (forall F d',
+      (F * pre)%pred d ->
+      exec o d p (Crashed d') ->
+      (F * crash)%pred d' ->
+      (F * augcrash o d)%pred d') ->
+  << o, d >>
+     pre
+     p
+  << r >>
+     (post r)
+     crash
+     (augpost o d r)
+     (augcrash o d).
+Proof.
+  unfold hoare_triple; intros.
+  edestruct H; eauto; cleanup.
+  
+  split_ors; cleanup.
+  - 
+    eexists; split; intuition eauto.
+    left; do 2 eexists; intuition eauto.
+    eapply H0; eauto.
+    pred_apply; cancel.
+    
+  - 
+    eexists; split; intuition eauto.
+    right; eexists; intuition eauto.
+    eapply H1; eauto.
+    pred_apply; cancel.
+Qed.
+
+End HoareLogic.
