src/Common/Primitives.v
@@ -1,3 +1,3 @@
 Require Export List BaseTypes Mem Pred SepAuto.
-Require Export Disk CommonAutomation ListUtils.
+Require Export Disk CommonAutomation ListUtils Common.HoareLogic.
 Export ListNotations.
