src/Layer1/Layer1.v
@@ -1,5 +1,5 @@
-Require Export HoareLogic Layer1.Specs ProgAuto.
-Require Export Layer1.Definitions Layer1.Facts.
+Require Export Layer1.Definitions Layer1.ProgAuto.
+Require Export  Layer1.Facts Layer1.HoareLogic Layer1.Specs.
 Notation "'Layer1.state'" := Layer1.Definitions.state.
 Notation "'Layer1.oracle'" := Layer1.Definitions.oracle.
 Notation "'Layer1.prog'" := Layer1.Definitions.prog.
@@ -9,3 +9,4 @@ Notation "'Layer1.Ret'" := Layer1.Definitions.Ret.
 Notation "'Layer1.Bind'" := Layer1.Definitions.Bind.
 Notation "'Layer1.Cont'" := Layer1.Definitions.Cont.
 Notation "'Layer1.Crash'" := Layer1.Definitions.Crash.
+Notation "'Layer1.oracle_ok'" := Layer1.Definitions.oracle_ok.
