src/Layer2/Layer2.v
@@ -3,3 +3,6 @@ Notation "'Layer2.state'" := Layer2.Definitions.state.
 Notation "'Layer2.oracle'" := Layer2.Definitions.oracle.
 Notation "'Layer2.prog'" := Layer2.Definitions.prog.
 Notation "'Layer2.exec'" := Layer2.Definitions.exec.
+Notation "'Layer2.Read'" := Layer2.Definitions.Read.
+Notation "'Layer2.Write'" := Layer2.Definitions.Write.
+Notation "'Layer2.Cont'" := Layer2.Definitions.Cont.
